SoftwareFoundations/SfLib/Types.v
@@ -39,3 +39,60 @@ Hint Resolve beq_id_eq beq_id_false_not_eq.
 Definition amultistep st := multi (astep st).
 
 Notation " t '/' st '=>a*' t' " := (amultistep st t t') (at level 40, st at level 39).
+
+Example astep_example1:
+  (APlus (ANum 3) (AMult (ANum 3) (ANum 4)))  / empty_state =>a* (ANum 15).
+Proof.
+  apply multi_step with (APlus (ANum 3) (ANum 12)).
+    apply AS_Plus2.
+      apply av_num.
+      apply AS_Mult.
+  apply multi_step with (ANum 15).
+    apply AS_Plus.
+  apply multi_refl.
+Qed.
+
+Hint Constructors astep aval.
+
+Example astep_example1':
+  (APlus (ANum 3) (AMult (ANum 3) (ANum 4)))  / empty_state =>a* (ANum 15).
+Proof.
+  eapply multi_step. auto. simpl.
+  eapply multi_step. auto. simpl.
+  apply multi_refl.
+Qed.
+
+Tactic Notation "print_goal" := match goal with |- ?x => idtac x end.
+Tactic Notation "normalize" := 
+   repeat (print_goal; eapply multi_step ; 
+             [ (eauto 10; fail) | (instantiate; simpl)]);
+   apply multi_refl.
+
+Example astep_example1'':
+  (APlus (ANum 3) (AMult (ANum 3) (ANum 4)))  / empty_state =>a* (ANum 15).
+Proof.
+  normalize.
+Qed.
+
+Example astep_example1''':
+  exists e', (APlus (ANum 3) (AMult (ANum 3) (ANum 4)))  / empty_state =>a* e'.
+Proof.
+  eapply ex_intro. normalize.
+Qed.
+
+Theorem normalize_ex:
+  exists e', (AMult (ANum 3) (AMult (ANum 2) (ANum 1))) / empty_state =>a* e'.
+Proof.
+  eapply ex_intro. normalize.
+Qed.
+
+Theorem normalize_ex':
+  exists e', (AMult (ANum 3) (AMult (ANum 2) (ANum 1))) / empty_state =>a* e'.
+Proof.
+  apply ex_intro with (ANum 6).
+  normalize.
+Qed.
+
+(*** Types Arithmetic Expressions ***)
+
+
